theories/prepost.v
@@ -3,6 +3,7 @@ Require Export iris.algebra.updates.
 Require Export iris.base_logic.base_logic.
 Require Export iris.proofmode.proofmode.
 Require Export refframe.module.
+Require Export refframe.satisfiable.
 Require Import refframe.trefines.
 Require Import refframe.link.
 Require Import refframe.seq_product.
@@ -11,148 +12,79 @@ Require Import refframe.proof_techniques.
 
 Set Default Proof Using "Type".
 
-Section updates.
-  Context {A : cmra}.
-  Lemma cmra_update_included (x y : A) :
-    x ≼ y → y ~~> x.
-  Proof. move => [? ->]. apply cmra_update_op_l. Qed.
-End updates.
-
-Section total_updates.
-  Local Set Default Proof Using "Type*".
-  Context {A : cmra}.
-  Lemma cmra_update_valid (x y : A) :
-    x ~~> y → ✓ x → ✓ y.
-  Proof.
-    move => Hupd /cmra_valid_validN Hvalid.
-    apply /cmra_valid_validN => n.
-    by apply (Hupd n None).
-  Qed.
-End total_updates.
-
-Section included.
-  Context {A : cmra}.
-  Implicit Types (x y z : A).
-  Lemma cmra_included_op_l x y z : x ≼ y → x ≼ y ⋅ z.
-  Proof. intros ?. etrans; [done|]. apply cmra_included_l. Qed.
-  Lemma cmra_included_op_r x y z : x ≼ y → x ≼ z ⋅ y.
-  Proof. intros ?. etrans; [done|]. apply cmra_included_r. Qed.
-End included.
-
-Section satisfiable.
-  Context {M : ucmra}.
-
-  Definition satisfiable (P: uPred M) := ∃ x : M, ✓{0} x ∧ uPred_holds P 0 x.
-
-  Global Instance satisfiable_proper : Proper ((≡) ==> iff) satisfiable.
-  Proof.
-    move => ?? Hequiv. unfold satisfiable. f_equiv => ?.
-    split => -[??]. all: split; [done|]. all: apply: uPred_holds_ne; [| |done..]; [|done]; by rewrite Hequiv.
-  Qed.
-
-  Lemma satisfiable_valid x:
-    satisfiable (uPred_ownM x) → ✓{0} x.
-  Proof. unfold satisfiable; uPred.unseal. move => [?[??]]. by apply: cmra_validN_includedN. Qed.
-
-  Lemma satisfiable_pure_1 (ϕ : Prop):
-    ϕ →
-    satisfiable ⌜ϕ⌝.
-  Proof. move => ?. unfold satisfiable; uPred.unseal. eexists ε. split; [|done]. apply ucmra_unit_validN. Qed.
-
-  Lemma satisfiable_pure_2 (ϕ : Prop):
-    satisfiable ⌜ϕ⌝ →
-    ϕ.
-  Proof. unfold satisfiable; uPred.unseal. naive_solver. Qed.
-
-  Lemma satisfiable_bupd_2 x:
-    satisfiable (|==> x) →
-    satisfiable x.
-  Proof.
-    unfold satisfiable; uPred.unseal.
-    move => -[x'[Hv HP]].
-    destruct (HP 0 ε) as [y HP']; [done|by rewrite right_id|].
-    move: HP'. rewrite right_id; eauto.
-  Qed.
-
-  Lemma satisfiable_mono x y:
-    satisfiable x →
-    (x ⊢ y) →
-    satisfiable y.
-  Proof. move => [?[??]] Hentails. eexists _. split; [done|]. by apply Hentails. Qed.
-
-  Lemma satisfiable_bmono x y:
-    satisfiable x →
-    (x ==∗ y) →
-    satisfiable y.
-  Proof. move => ??. apply satisfiable_bupd_2. by apply: satisfiable_mono. Qed.
-End satisfiable.
-
 (** * prepost *)
 Section prepost.
 Context {R : Type}.
 Context {M : ucmra}.
 
+
 Inductive prepost : Type :=
 | pp_end (r : R)
 | pp_prop (P : Prop) (pp : prepost)
 | pp_quant {T} (pp : T → prepost)
-| pp_add (P : uPred M) (pp : prepost)
-| pp_remove (P : uPred M) (pp : prepost)
-(* | pp_update (pp : prepost) *)
+| pp_star (P : uPred M) (pp : prepost)
 .
 
-Fixpoint pp_to_ex (pp : prepost) (x : uPred M) (Q : R → uPred M → Prop) : Prop :=
+Fixpoint pp_to_ex (pp : prepost) (Q : R → uPred M → Prop) : Prop :=
   match pp with
-  | pp_end r => Q r x
-  | pp_prop P pp' => P ∧ pp_to_ex pp' x Q
-  | pp_quant pp' => ∃ y, pp_to_ex (pp' y) x Q
-  | pp_add P pp' => satisfiable (P ∗ x) ∧ pp_to_ex pp' (P ∗ x) Q
-  (* We could also put and ≡ here but that makes it more annoying for
-  the users because they probably always want an update. *)
-  | pp_remove P pp' => ∃ y, (x ==∗ (P ∗ y)) ∧ pp_to_ex pp' y Q
-  (* | pp_update pp' => ∃ y, x ~~> y ∧ pp_to_ex pp' y Q *)
+  | pp_end r => Q r True%I
+  | pp_prop P pp' => P ∧ pp_to_ex pp' Q
+  | pp_quant pp' => ∃ y, pp_to_ex (pp' y) Q
+  | pp_star P pp' => pp_to_ex pp' (λ r y, Q r (P ∗ y)%I)
   end.
 
-Fixpoint pp_to_all (pp : prepost) (x : uPred M) (Q : R → uPred M → Prop) : Prop :=
+Fixpoint pp_to_all (pp : prepost) (Q : R → uPred M → Prop) : Prop :=
   match pp with
-  | pp_end r => Q r x
-  | pp_prop P pp' => P → pp_to_all pp' x Q
-  | pp_quant pp' => ∀ y, pp_to_all (pp' y) x Q
-  | pp_add P pp' => satisfiable (P ∗ x) → pp_to_all pp' (P ∗ x) Q
-  | pp_remove P pp' => ∀ y, (x ==∗ P ∗ y) → pp_to_all pp' y Q
-  (* | pp_update pp' => ∀ y, x ~~> y → pp_to_all pp' y Q *)
+  | pp_end r => Q r True%I
+  | pp_prop P pp' => P → pp_to_all pp' Q
+  | pp_quant pp' => ∀ y, pp_to_all (pp' y) Q
+  | pp_star P pp' => pp_to_all pp' (λ r y, Q r (P ∗ y)%I)
   end.
 
-Lemma pp_to_ex_exists pp Q x:
-  pp_to_ex pp x Q ↔ ∃ r y, Q r y ∧ pp_to_ex pp x (λ r' y', r' = r ∧ y' = y).
-Proof. elim: pp x => /=; naive_solver. Qed.
+Lemma pp_to_ex_exists pp Q:
+  pp_to_ex pp Q ↔ ∃ r y, Q r y ∧ pp_to_ex pp (λ r' y', r' = r ∧ y' = y).
+Proof.
+  elim: pp Q => /=; try naive_solver.
+  move => ?? IH Q. rewrite IH.
+  split; move => [?[?[? Hex]]].
+  - eexists _, _. split; [done|]. rewrite IH. naive_solver.
+  - move: Hex. rewrite IH. naive_solver.
+Qed.
 
-Lemma pp_to_all_forall pp Q x:
-  pp_to_all pp x Q ↔ (∀ r y, pp_to_ex pp x (λ r' y', r' = r ∧ y' = y) → Q r y).
-Proof. elim: pp x => /=; naive_solver. Qed.
-Lemma pp_to_all_forall_2 pp Q x:
-  pp_to_all pp x Q →
-  ∀ r y, pp_to_ex pp x (λ r' y', r' = r ∧ y' = y) → Q r y.
+Lemma pp_to_all_forall pp Q:
+  pp_to_all pp Q ↔ (∀ r y, pp_to_ex pp (λ r' y', r' = r ∧ y' = y) → Q r y).
+Proof.
+  elim: pp Q => /=; try naive_solver.
+  move => ?? IH Q. rewrite IH.
+  split; move => Hall ??.
+  - rewrite pp_to_ex_exists => -[?[?[??]]]. naive_solver.
+  - move => ?. apply Hall. rewrite pp_to_ex_exists. naive_solver.
+Qed.
+
+Lemma pp_to_all_forall_2 pp Q:
+  pp_to_all pp Q →
+  ∀ r y, pp_to_ex pp (λ r' y', r' = r ∧ y' = y) → Q r y.
 Proof. apply pp_to_all_forall. Qed.
 
-Lemma pp_to_all_mono pp (Q1 Q2 : _ → _ → Prop) x:
-  pp_to_all pp x Q1 →
+Lemma pp_to_all_mono pp (Q1 Q2 : _ → _ → Prop):
+  pp_to_all pp Q1 →
   (∀ r y, Q1 r y → Q2 r y) →
-  pp_to_all pp x Q2.
-Proof. elim: pp x => /=; naive_solver. Qed.
+  pp_to_all pp Q2.
+Proof. rewrite !pp_to_all_forall. naive_solver. Qed.
 
-Lemma pp_to_ex_mono pp (Q1 Q2 : _ → _ → Prop) x:
-  pp_to_ex pp x Q1 →
+Lemma pp_to_ex_mono pp (Q1 Q2 : _ → _ → Prop):
+  pp_to_ex pp Q1 →
   (∀ r y, Q1 r y → Q2 r y) →
-  pp_to_ex pp x Q2.
-Proof. elim: pp x => /=; naive_solver. Qed.
+  pp_to_ex pp Q2.
+Proof. rewrite !pp_to_ex_exists. naive_solver. Qed.
 
-Lemma pp_to_all_ex pp Q1 Q2 x:
-  pp_to_all pp x Q1 →
-  pp_to_ex pp x Q2 →
+Lemma pp_to_all_ex pp Q1 Q2:
+  pp_to_all pp Q1 →
+  pp_to_ex pp Q2 →
   ∃ y r, Q1 r y ∧ Q2 r y.
 Proof. move => /pp_to_all_forall ? /pp_to_ex_exists. naive_solver. Qed.
 
+(*
 Definition pp_res_equiv (Q : R → uPred M → Prop) (r : R) (x : uPred M) : Prop :=
   ∀ x', satisfiable x' → x' ≡ x → Q r x'.
 
@@ -191,6 +123,7 @@ Proof.
     apply: satisfiable_bmono; [done|]. rewrite Hequiv. etrans; [done|].
     by iIntros ">[_ $]".
 Qed.
+*)
 
 (*
 Definition pp_res_upd (Q : R → A → Prop) (r : R) (x : A) : Prop :=
@@ -287,14 +220,16 @@ Section prepost.
   | PPOutsideS s x e:
     pp_filter_step i o (PPOutside, s, x) (Some (inr e)) (λ σ, σ = (PPRecv1 e, s, x))
   | PPRecv1S s x e:
-    pp_filter_step i o (PPRecv1 e, s, x) None (λ σ, pp_to_ex (i e s) x (λ r y, σ = (PPRecv2 r.1, r.2, y)))
+    pp_filter_step i o (PPRecv1 e, s, x) None (λ σ,
+        pp_to_ex (i e s) (λ r y, ∃ x', satisfiable (x ∗ y ∗ x') ∧ σ = (PPRecv2 r.1, r.2, x')))
   | PPRecv2S s x e:
     pp_filter_step i o (PPRecv2 e, s, x) (Some (inl e)) (λ σ, σ = (PPInside, s, x))
   | PPInsideS s x e:
     pp_filter_step i o (PPInside, s, x) (Some (inl e)) (λ σ, σ = (PPSend1 e, s, x))
-  | PPSend1S s x e r y:
-    pp_to_ex (o e s) x (λ r' y', r' = r ∧ y' = y) →
-    pp_filter_step i o (PPSend1 e, s, x) None (λ σ, σ = (PPSend2 r.1, r.2, y))
+  | PPSend1S s x e r y x':
+    satisfiable (x' ∗ y ∗ x) →
+    pp_to_ex (o e s) (λ r' y', r' = r ∧ y' = y) →
+    pp_filter_step i o (PPSend1 e, s, x) None (λ σ, σ = (PPSend2 r.1, r.2, x'))
   | PPSend2S s x e:
     pp_filter_step i o (PPSend2 e, s, x) (Some (inr e)) (λ σ, σ = (PPOutside, s, x))
   .
@@ -329,9 +264,10 @@ Section prepost.
 
   Lemma mod_prepost_step_Recv1_i i o m σ s e x:
     TStepI (mod_prepost i o m) (SMFilter, σ, (PPRecv1 e, s, x)) (λ G,
-        pp_to_ex (i e s) x (λ r y, G true None (λ G', G' (SMProgRecv r.1, σ, (PPInside, r.2, y))))).
+        pp_to_ex (i e s) (λ r y, ∃ x', satisfiable (x ∗ y ∗ x') ∧
+                      G true None (λ G', G' (SMProgRecv r.1, σ, (PPInside, r.2, x'))))).
   Proof.
-    constructor => G /= /pp_to_ex_exists[r [HG Hex]]. tstep_i.
+    constructor => G /= /pp_to_ex_exists[r [? [[?[? HG]]?]]]. tstep_i.
     apply steps_impl_step_next => ???. invert_all @m_step.
     eexists (_, _). split!. { apply pp_to_ex_exists. naive_solver. }
     apply steps_impl_step_end => ???. invert_all @m_step => ???. naive_solver.
@@ -339,15 +275,16 @@ Section prepost.
 
   Lemma mod_prepost_step_Inside_i i o m σ s e x:
     TStepI (mod_prepost i o m) (SMFilterRecv e, σ, (PPInside, s, x)) (λ G,
-        pp_to_all (o e s) x (λ r y, G true (Some (r.1)) (λ G', G' (SMFilter, σ, (PPOutside, r.2, y))))).
+        pp_to_all (o e s) (λ r y, ∀ x', satisfiable (x' ∗ y ∗ x) →
+            G true (Some (r.1)) (λ G', G' (SMFilter, σ, (PPOutside, r.2, x'))))).
   Proof.
     constructor => G /= ?. apply steps_impl_step_trans. tstep_i.
     apply steps_impl_step_end => ???. invert_all @m_step => ? b *; simplify_eq. split! => ?. split!; [done|].
     tstep_i.
     apply steps_impl_step_next => ???. invert_all @m_step => *; simplify_eq. split!.
     apply steps_impl_step_end => ???. invert_all @m_step => *; simplify_eq. split! => ?.
-    have [?[?[?[??]]]]:= pp_to_all_ex _ _ _ _ ltac:(done) ltac:(done); subst.
-    split!; [done|by destruct b|]. naive_solver.
+    have [?[?[?[??]]]]:= pp_to_all_ex _ _ _ ltac:(done) ltac:(done); subst.
+    split!; [naive_solver|by destruct b|]. naive_solver.
   Qed.
 
   Lemma mod_prepost_step_Outside_s i o m σ s x:
@@ -361,26 +298,28 @@ Section prepost.
 
   Lemma mod_prepost_step_Recv1_s i o m σ s e x:
     TStepS (mod_prepost i o m) (SMFilter, σ, (PPRecv1 e, s, x)) (λ G,
-        G None (λ G', pp_to_all (i e s) x (λ r y, G' (SMProgRecv r.1, σ, (PPInside, r.2, y))))).
+        G None (λ G', pp_to_all (i e s) (λ r y, ∀ x', satisfiable (x ∗ y ∗ x') →
+             G' (SMProgRecv r.1, σ, (PPInside, r.2, x'))))).
   Proof.
     constructor => G /= ?. split!; [done|] => /= ??. apply steps_spec_step_trans.
     tstep_s. eexists None. split!.
     apply: steps_spec_step_end; [by econs|] => ? /=?.
-    have [?[?[??]]]:= pp_to_all_ex _ _ _ _ ltac:(done) ltac:(done); subst.
+    have [?[?[?[?[??]]]]]:= pp_to_all_ex _ _ _ ltac:(done) ltac:(done); subst.
     tstep_s. eexists (Some (inl _)). split!.
-    apply: steps_spec_step_end; [by econs|]. naive_solver.
+    apply: steps_spec_step_end; [econs|]. naive_solver.
   Qed.
 
   Lemma mod_prepost_step_Inside_s i o m σ s e x:
     TStepS (mod_prepost i o m) (SMFilterRecv e, σ, (PPInside, s, x)) (λ G,
-        pp_to_ex (o e s) x (λ r y, G (Some (r.1)) (λ G', G' (SMFilter, σ, (PPOutside, r.2, y))))).
+        pp_to_ex (o e s) (λ r y, ∃ x', satisfiable (x' ∗ y ∗ x) ∧
+           G (Some (r.1)) (λ G', G' (SMFilter, σ, (PPOutside, r.2, x'))))).
   Proof.
-    constructor => G /= /pp_to_ex_exists[?[?[??]]]. split!; [done|] => /= ??.
+    constructor => G /= /pp_to_ex_exists[?[?[[?[??]]?]]]. split!; [done|] => /= ??.
     apply steps_spec_step_trans. tstep_s. eexists (Some _). split!.
     apply: steps_spec_step_end; [by econs|] => /= ? ->. tstep_s. eexists (Some (inr _)). split!.
     apply: steps_spec_step; [by econs|] => /= ? ->.
     apply: steps_spec_step_end; [by econs|] => /= ? ->.
-    done.
+    naive_solver.
   Qed.
 End prepost.
 
@@ -404,14 +343,14 @@ Proof.
   apply tsim_implies_trefines => /= n.
   tstep_i => ?.
   tstep_s. split!.
-  tstep_s. apply pp_to_all_forall => ???.
+  tstep_s. apply pp_to_all_forall => ?????.
   tstep_i. apply: pp_to_ex_mono; [done|].
-  move => ?? [<- <-].
+  move => ?? [? ?]. subst. eexists _. split; [done|].
   tstep_i => ? <-.
-  tstep_i.
+  tstep_i. eexists True%I. split. { apply satisfiable_emp_valid. by iSplit. }
   unshelve apply: tsim_remember. { simpl. exact (λ _
-      '(σf1, (σf1', σ1, (σpp1', _, _)), (σpp1, s1, x1)) '(σf2, σ2, (σpp2, s2, x2)),
-         σf1 = SMProg ∧ σf1' = σf2 ∧ σ1 = σ2 ∧ σpp1 = PPInside ∧ x1 = x2
+      '(σf1, (σf1', σ1, (σpp1', _, x')), (σpp1, s1, x1)) '(σf2, σ2, (σpp2, s2, x2)),
+         x' = True%I ∧ σf1 = SMProg ∧ σf1' = σf2 ∧ σ1 = σ2 ∧ σpp1 = PPInside ∧ x1 = x2
          ∧ σpp1' = PPInside ∧ σpp2 = PPInside ∧ s1 = s2 ∧
          ((∃ e, σf1' = SMProgRecv e) ∨ σf1' = SMProg)). }
   { split!. } { done. }
@@ -426,14 +365,14 @@ Proof.
   - tstep_both. apply: steps_impl_step_end => κ ??.
     tstep_s. eexists _. apply: steps_spec_step_end; [done|] => ??.
     case_match; tend; (split!; [done|]). 2: { apply: Hloop; [done|]. split!. }
-    tstep_i. tstep_i. apply pp_to_all_forall => ???.
-    tstep_s. apply: pp_to_ex_mono; [done|]. move => ?? [<- <-]. split!.
+    tstep_i => ??. tstep_i. apply pp_to_all_forall => ?????.
+    tstep_s. apply: pp_to_ex_mono; [done|]. move => ?? [? ?]. split!; subst; [done..|].
     tstep_i => ?.
     tstep_s. split!.
-    tstep_s. apply pp_to_all_forall => ???.
-    tstep_i. apply: pp_to_ex_mono; [done|]. move => ?? [<- <-].
+    tstep_s. apply pp_to_all_forall => ?????.
+    tstep_i. apply: pp_to_ex_mono; [done|]. move => ?? [??]; subst. split!; [done|].
     tstep_i => ? <-.
-    tstep_i.
+    tstep_i. split!; [done|].
     apply Hloop; [done|]. split!.
 Qed.
 
@@ -449,7 +388,7 @@ Section prepost.
   Lemma mod_prepost_link
         {EV1 EV2 S1 S2 S' Sr1 Sr2 : Type}
         {M : ucmra}
-        (INV : seq_product_state → S1 → S2 → S' → uPred M → uPred M → Sr1 → Sr2 → Prop)
+        (INV : seq_product_state → S1 → S2 → S' → uPred M → uPred M → uPred M → Sr1 → Sr2 → Prop)
         (i1 : io_event EV2 → S1 → prepost (io_event EV1 * S1) M)
         (o1 : io_event EV1 → S1 → prepost (io_event EV2 * S1) M)
         (i2 : io_event EV2 → S2 → prepost (io_event EV1 * S2) M)
@@ -464,151 +403,137 @@ Section prepost.
         :
 
        (∀ p s e p' s' e', R1 p s e p' s' e' → p ≠ p') →
-       (x ⊣⊢ x1 ∗ x2) →
-       satisfiable x →
-       INV SPNone s1 s2 s x1 x2 sr1 sr2 →
-       (∀ s1 s2 s x1 x2 sr1 sr2 e sr1' e',
-          INV SPNone s1 s2 s x1 x2 sr1 sr2 →
-          satisfiable (x1 ∗ x2) →
+       INV SPNone s1 s2 s x1 x2 x sr1 sr2 →
+       (∀ s1 s2 s x1 x2 x sr1 sr2 e sr1' e',
+          INV SPNone s1 s2 s x1 x2 x sr1 sr2 →
           R1 SPNone sr1 e SPLeft sr1' e' →
-          pp_to_all (i (Incoming, e') s) (x1 ∗ x2) (λ r1 y1,
-          pp_to_ex (i1 (Incoming, e') s1) x1 (λ r2 y2, ∃ e sr2',
+          pp_to_all (i (Incoming, e') s) (λ r1 y1,
+          ∀ x', satisfiable (x ∗ y1 ∗ x') →
+          pp_to_ex (i1 (Incoming, e') s1) (λ r2 y2, ∃ e sr2' x'2,
+            satisfiable (x1 ∗ y2 ∗ x'2) ∧
             r1.1.1 = Incoming ∧
             r2.1.1 = Incoming ∧
             r1.1.2 = r2.1.2 ∧
-            (y1 ==∗ y2 ∗ x2) ∧
             R2 SPNone sr2 e SPLeft sr2' r1.1.2 ∧
-            INV SPLeft r2.2 s2 r1.2 y2 x2 sr1' sr2'))) →
-       (∀ s1 s2 s x1 x2 sr1 sr2 e sr1' e',
-          INV SPNone s1 s2 s x1 x2 sr1 sr2 →
-          satisfiable (x1 ∗ x2) →
+            INV SPLeft r2.2 s2 r1.2 x'2 x2 x' sr1' sr2'))) →
+       (∀ s1 s2 s x1 x2 x sr1 sr2 e sr1' e',
+          INV SPNone s1 s2 s x1 x2 x sr1 sr2 →
           R1 SPNone sr1 e SPRight sr1' e' →
-          pp_to_all (i (Incoming, e') s) (x1 ∗ x2) (λ r1 y1,
-          pp_to_ex (i2 (Incoming, e') s2) x2 (λ r2 y2, ∃ e sr2',
+          pp_to_all (i (Incoming, e') s) (λ r1 y1,
+          ∀ x', satisfiable (x ∗ y1 ∗ x') →
+          pp_to_ex (i2 (Incoming, e') s2) (λ r2 y2, ∃ e sr2' x'2,
+            satisfiable (x2 ∗ y2 ∗ x'2) ∧
             r1.1.1 = Incoming ∧
             r2.1.1 = Incoming ∧
             r1.1.2 = r2.1.2 ∧
-            (y1 ==∗ x1 ∗ y2) ∧
             R2 SPNone sr2 e SPRight sr2' r1.1.2 ∧
-            INV SPRight s1 r2.2 r1.2 x1 y2 sr1' sr2'))) →
-       (∀ s1 s2 s x1 x2 sr1 sr2 e,
-           INV SPLeft s1 s2 s x1 x2 sr1 sr2 →
-           satisfiable (x1 ∗ x2) →
-           pp_to_all (o1 e s1) x1 (λ r1 y1, ∀ sr1' e',
+            INV SPRight s1 r2.2 r1.2 x1 x'2 x' sr1' sr2'))) →
+       (∀ s1 s2 s x1 x2 x sr1 sr2 e,
+           INV SPLeft s1 s2 s x1 x2 x sr1 sr2 →
+           pp_to_all (o1 e s1) (λ r1 y1, ∀ sr1' e' x',
+             satisfiable (x' ∗ y1 ∗ x1) →
              r1.1.1 = Outgoing →
              R1 SPLeft sr1 r1.1.2 SPRight sr1' e' →
-             pp_to_ex (i2 (Incoming, e') s2) x2 (λ r2 y2, ∃ sr2',
+             pp_to_ex (i2 (Incoming, e') s2) (λ r2 y2, ∃ sr2' x'2,
+               satisfiable (x2 ∗ y2 ∗ x'2) ∧
                e.1 = Outgoing ∧
                r2.1.1 = Incoming ∧
-               (x1 ∗ x2 ==∗ y1 ∗ y2) ∧
-               INV SPRight r1.2 r2.2 s y1 y2 sr1' sr2' ∧
+               INV SPRight r1.2 r2.2 s x' x'2 x sr1' sr2' ∧
                R2 SPLeft sr2 e.2 SPRight sr2' r2.1.2))) →
-       (∀ s1 s2 s x1 x2 sr1 sr2 e,
-           INV SPLeft s1 s2 s x1 x2 sr1 sr2 →
-           satisfiable (x1 ∗ x2) →
-           ∀ x, (x ==∗ (x1 ∗ x2)) →
-           pp_to_all (o1 e s1) x1 (λ r1 y1, ∀ sr1' e',
+       (∀ s1 s2 s x1 x2 x sr1 sr2 e,
+           INV SPLeft s1 s2 s x1 x2 x sr1 sr2 →
+           pp_to_all (o1 e s1) (λ r1 y1, ∀ sr1' e' x',
+             satisfiable (x' ∗ y1 ∗ x1) →
              r1.1.1 = Outgoing →
              R1 SPLeft sr1 r1.1.2 SPNone sr1' e' →
              ∃ e'' sr2',
                e.1 = Outgoing ∧
                R2 SPLeft sr2 e.2 SPNone sr2' e'' ∧
-               pp_to_ex (o (Outgoing, e'') s) x (λ r2 y2,
+               pp_to_ex (o (Outgoing, e'') s) (λ r2 y2, ∃ x'2,
+                 satisfiable (x'2 ∗ y2 ∗ x) ∧
                  r2.1.1 = Outgoing ∧
                  r2.1.2 = e' ∧
-                 (* This = instead of ≡ is fine because the pp_to_ex
-                 must have a update in it. *)
-                 y2 = (y1 ∗ x2)%I ∧
-                 INV SPNone r1.2 s2 r2.2 y1 x2 sr1' sr2'))) →
-       (∀ s1 s2 s x1 x2 sr1 sr2 e,
-           INV SPRight s1 s2 s x1 x2 sr1 sr2 →
-           satisfiable (x1 ∗ x2) →
-           pp_to_all (o2 e s2) x2 (λ r1 y1, ∀ sr1' e',
+                 INV SPNone r1.2 s2 r2.2 x' x2 x'2 sr1' sr2'))) →
+       (∀ s1 s2 s x1 x2 x sr1 sr2 e,
+           INV SPRight s1 s2 s x1 x2 x sr1 sr2 →
+           pp_to_all (o2 e s2) (λ r1 y1, ∀ sr1' e' x',
+             satisfiable (x' ∗ y1 ∗ x2) →
              r1.1.1 = Outgoing →
              R1 SPRight sr1 r1.1.2 SPLeft sr1' e' →
-             pp_to_ex (i1 (Incoming, e') s1) x1 (λ r2 y2, ∃ sr2',
+             pp_to_ex (i1 (Incoming, e') s1) (λ r2 y2, ∃ sr2' x'2,
+               satisfiable (x1 ∗ y2 ∗ x'2) ∧
                e.1 = Outgoing ∧
                r2.1.1 = Incoming ∧
-               (x1 ∗ x2 ==∗ y2 ∗ y1) ∧
-               INV SPLeft r2.2 r1.2 s y2 y1 sr1' sr2' ∧
+               INV SPLeft r2.2 r1.2 s x'2 x' x sr1' sr2' ∧
                R2 SPRight sr2 e.2 SPLeft sr2' r2.1.2))) →
-       (∀ s1 s2 s x1 x2 sr1 sr2 e,
-           INV SPRight s1 s2 s x1 x2 sr1 sr2 →
-           satisfiable (x1 ∗ x2) →
-           ∀ x, (x ==∗ (x1 ∗ x2)) →
-           pp_to_all (o2 e s2) x2 (λ r1 y1, ∀ sr1' e',
+       (∀ s1 s2 s x1 x2 x sr1 sr2 e,
+           INV SPRight s1 s2 s x1 x2 x sr1 sr2 →
+           pp_to_all (o2 e s2) (λ r1 y1, ∀ sr1' e' x',
+             satisfiable (x' ∗ y1 ∗ x2) →
              r1.1.1 = Outgoing →
              R1 SPRight sr1 r1.1.2 SPNone sr1' e' →
              ∃ e'' sr2',
                e.1 = Outgoing ∧
                R2 SPRight sr2 e.2 SPNone sr2' e'' ∧
-               pp_to_ex (o (Outgoing, e'') s) x (λ r2 y2,
+               pp_to_ex (o (Outgoing, e'') s) (λ r2 y2, ∃ x'2,
+                 satisfiable (x'2 ∗ y2 ∗ x) ∧
                  r2.1.1 = Outgoing ∧
                  r2.1.2 = e' ∧
-                 (* This = instead of ≡ is fine because the pp_to_ex
-                 must have a update in it. *)
-                 y2 = (x1 ∗ y1)%I ∧
-                 INV SPNone s1 r1.2 r2.2 x1 y1 sr1' sr2'))) →
+                 INV SPNone s1 r1.2 r2.2 x1 x' x'2 sr1' sr2'))) →
     trefines (MS (mod_link R1 (mod_prepost i1 o1 m1) (mod_prepost i2 o2 m2))
                  (MLFNone, sr1, (SMFilter, σ1, (PPOutside, s1, x1)), (SMFilter, σ2, (PPOutside, s2, x2))))
              (MS (mod_prepost i o (mod_link R2 m1 m2))
                  (SMFilter, (MLFNone, sr2, σ1, σ2), (PPOutside, s, x))).
     Proof.
-      move => Hneq Hequiv Hvalid Hinv HN2L HN2R HL2R HL2N HR2L HR2N.
+      move => Hneq Hinv HN2L HN2R HL2R HL2N HR2L HR2N.
       apply tsim_implies_trefines => /= n.
       unshelve apply: tsim_remember. { simpl. exact (λ _
           '(σl1, sr1, (σf1, σ1, (σpp1, s1, x1)), (σf2, σ2, (σpp2, s2, x2)))
           '(σf, (σl2, sr2, σ1', σ2'), (σpp, s, x)),
            ∃ sp,
-           σ1 = σ1' ∧ σ2 = σ2' ∧ INV sp s1 s2 s x1 x2 sr1 sr2 ∧ satisfiable x ∧
-          (* Here we have an ≡ instead of a ==∗ since we know that the
-          resources in the spec must be up to date because the last
-          interaction was with the environment *)
-          (( sp = SPNone ∧ (x ⊣⊢ x1 ∗ x2) ∧
+           σ1 = σ1' ∧ σ2 = σ2' ∧ INV sp s1 s2 s x1 x2 x sr1 sr2 ∧
+          (( sp = SPNone ∧
               σl1 = MLFNone ∧ σf = SMFilter
             ∧ σpp1 = PPOutside ∧ σpp2 = PPOutside ∧ σpp = PPOutside
             ∧ σf1 = SMFilter ∧ σf2 = SMFilter
             ∧ σl2 = MLFNone)
-           ∨ (sp = SPLeft ∧ (x ==∗ x1 ∗ x2) ∧
+           ∨ (sp = SPLeft ∧
               ((∃ e, σl2 = MLFRecvL e ∧ σf1 = SMProgRecv (Incoming, e))
                ∨ (σl2 = MLFLeft ∧ σf1 = SMProg))
             ∧ σpp1 = PPInside ∧ σpp2 = PPOutside ∧ σpp = PPInside
             ∧ σf = SMProg ∧ σf2 = SMFilter
             ∧ σl1 = MLFLeft)
-           ∨ (sp = SPRight ∧ (x ==∗ x1 ∗ x2) ∧
+           ∨ (sp = SPRight ∧
               ((∃ e, σl2 = MLFRecvR e ∧ σf2 = SMProgRecv (Incoming, e))
                ∨ (σl2 = MLFRight ∧ σf2 = SMProg))
             ∧ σpp1 = PPOutside ∧ σpp2 = PPInside ∧ σpp = PPInside
             ∧ σf = SMProg ∧ σf1 = SMFilter
             ∧ σl1 = MLFRight) )). }
       { split!. } { done. }
-      move => {}n _ /= Hloop {Hinv Hequiv Hvalid}.
+      move => {}n _ /= Hloop {Hinv}.
       move => [[[σl1 {}sr1] [[σf1 {}σ1] [[σpp1 {}s1] {}x1]]] [[σf2 {}σ2] [[σpp2 {}s2] {}x2]]].
       move => [[σf [[[σl2 {}sr2] σ1'] σ2']] [[σpp {}s] {}x]] ?. destruct_all?; simplify_eq.
-      - revert select (satisfiable x) => Hvalid. revert select (x ⊣⊢ _) => Hequiv.
-        move: (Hvalid) => Hvalid2. rewrite Hequiv in Hvalid2.
-        tstep_i => ? p' ???.
+      - tstep_i => ? p' ???.
         tstep_s. split!.
-        tstep_s. apply pp_to_all_forall => ri xi Hi.
+        tstep_s. apply pp_to_all_forall => ri xi Hi x' Hsat.
         destruct p' => /=. 3: naive_solver.
         + tstep_i => ??. simplify_eq.
-          tstep_i. move: ri xi Hi. apply pp_to_all_forall.
-          apply: pp_to_all_mono_res; [done..|].
+          tstep_i. move: ri xi Hi x' Hsat. apply: pp_to_all_forall_2.
           apply: pp_to_all_mono; [by apply: HN2L|].
-          move => [[??]?] ? /= Hcont ? ? Hequiv2. apply: pp_to_ex_mono; [done|].
-          move => [[??]?] ? /= *. destruct_all?; simplify_eq.
+          move => [[??]?] ? /= Hcont ??.
+          apply: pp_to_ex_mono; [naive_solver|].
+          move => [[??]?] ? /= *. destruct_all?; simplify_eq. split!; [done|].
           tstep_s.
           split!; [done..|] => /=.
-          apply: Hloop; [done|]. split!. by rewrite Hequiv2.
+          apply: Hloop; [done|]. split!.
         + tstep_i => ??. simplify_eq.
-          tstep_i. move: ri xi Hi. apply pp_to_all_forall.
-          apply: pp_to_all_mono_res; [done..|].
+          tstep_i. move: ri xi Hi x' Hsat. apply: pp_to_all_forall_2.
           apply: pp_to_all_mono; [by apply: HN2R|].
-          move => [[??]?] ? /= Hcont ? ? Hequiv2. apply: pp_to_ex_mono; [done|].
-          move => [[??]?] ? /= *. destruct_all?; simplify_eq.
+          move => [[??]?] ? /= Hcont ? ?. apply: pp_to_ex_mono; [naive_solver|].
+          move => [[??]?] ? /= *. destruct_all?; simplify_eq. split!; [done|].
           tstep_s.
           split!; [done..|] => /=.
-          apply: Hloop; [done|]. split!. by rewrite Hequiv2.
+          apply: Hloop; [done|]. split!.
       - tstep_both.
         apply steps_impl_step_end => κ Pσ2 ?. case_match; intros; simplify_eq.
         + tstep_s. eexists (Some (Incoming, _)). split!.
@@ -624,33 +549,30 @@ Section prepost.
           apply: Hloop; [done|]. by split!.
         }
         tend. have [σ' Hσ'] := vis_no_all _ _ _ ltac:(done). eexists σ'. split; [naive_solver|].
-        tstep_i. apply pp_to_all_forall => ri xi Hi p' sr1' e' HR1 Hri.
-        have ?:= satisfiable_bmono _ _ ltac:(done) ltac:(done).
+        tstep_i. apply pp_to_all_forall => ri xi Hi x' Hsat p' sr1' e' HR1 Hri.
         destruct p' => /=. 1: naive_solver.
         + tstep_i => ??; simplify_eq.
           tstep_i.
-          move: ri xi Hi sr1' e' Hri HR1. apply: pp_to_all_forall_2.
+          move: ri xi Hi x' Hsat sr1' e' Hri HR1. apply: pp_to_all_forall_2.
           apply: pp_to_all_mono; [by apply: HL2R|].
-          move => [[??]?] ? /= Hcont ????.
-          apply: pp_to_ex_mono; [ by apply: Hcont|].
-          move => [[??]?] ? /=?. destruct_all?; simplify_eq.
+          move => [[??]?] ? /= Hcont ??????.
+          apply: pp_to_ex_mono; [by apply: Hcont|].
+          move => [[??]?] ? /=?. destruct_all?; simplify_eq. split!; [done|].
           tstep_s. eexists (Some (Outgoing, _)). split!; [done|].
           destruct e; simplify_eq/=.
           apply: steps_spec_step_end; [done|] => ??.
-          apply: Hloop; [done|]. split!; [naive_solver|done..| ].
-          etrans; [done|]. etrans; [|apply bupd_trans]. by apply bupd_mono.
-        + move: ri xi Hi sr1' e' Hri HR1. apply: pp_to_all_forall_2.
+          apply: Hloop; [done|]. split!. naive_solver.
+        + move: ri xi Hi x' Hsat sr1' e' Hri HR1. apply: pp_to_all_forall_2.
           apply: pp_to_all_mono; [by apply: HL2N|].
-          move => [[??]?] ? /= Hcont ????.
-          have {}Hcont := Hcont _ _ ltac:(done) ltac:(done). destruct_all?.
+          move => [[??]?] ? /= Hcont ??????.
+          have {}Hcont := Hcont _ _ _ ltac:(done) ltac:(done) ltac:(done). destruct_all?.
           destruct e; simplify_eq/=.
           tstep_s. eexists (Some (Outgoing, _)). split!; [done|].
           apply: steps_spec_step_end; [done|] => ??.
           tstep_s.
-          apply: pp_to_ex_mono_res; [done..|].
           apply: pp_to_ex_mono; [done|].
-          move => [[??]?] ? /= ????. destruct_all?; simplify_eq. split!.
-          apply: Hloop; [done|]. split!; [naive_solver|done..].
+          move => [[??]?] ? /=?. destruct_all?; simplify_eq. split!; [done|].
+          apply: Hloop; [done|]. split!. naive_solver.
       - tstep_both.
         apply steps_impl_step_end => κ Pσ2 ?. case_match; intros; simplify_eq.
         + tstep_s. eexists (Some (Incoming, _)). split!.
@@ -666,33 +588,30 @@ Section prepost.
           apply: Hloop; [done|]. by split!.
         }
         tend. have [σ' Hσ'] := vis_no_all _ _ _ ltac:(done). eexists σ'. split; [naive_solver|].
-        tstep_i. apply pp_to_all_forall => ri xi Hi p' sr1' e' HR1 Hri.
-        have ?:= satisfiable_bmono _ _ ltac:(done) ltac:(done).
+        tstep_i. apply pp_to_all_forall => ri xi Hi x' Hsat p' sr1' e' HR1 Hri.
         destruct p' => /=. 2: naive_solver.
         + tstep_i => ??; simplify_eq.
           tstep_i.
-          move: ri xi Hi sr1' e' Hri HR1. apply: pp_to_all_forall_2.
+          move: ri xi Hi x' Hsat sr1' e' Hri HR1. apply: pp_to_all_forall_2.
           apply: pp_to_all_mono; [by apply: HR2L|].
-          move => [[??]?] ? /= Hcont ????.
-          apply: pp_to_ex_mono; [ by apply: Hcont|].
-          move => [[??]?] ? /=?. destruct_all?; simplify_eq.
+          move => [[??]?] ? /= Hcont ??????.
+          apply: pp_to_ex_mono; [by apply: Hcont|].
+          move => [[??]?] ? /=?. destruct_all?; simplify_eq. split!; [done|].
           tstep_s. eexists (Some (Outgoing, _)). split!; [done|].
           destruct e; simplify_eq/=.
           apply: steps_spec_step_end; [done|] => ??.
-          apply: Hloop; [done|]. split!; [naive_solver|done..| ].
-          etrans; [done|]. etrans; [|apply bupd_trans]. by apply bupd_mono.
-        + move: ri xi Hi sr1' e' Hri HR1. apply: pp_to_all_forall_2.
+          apply: Hloop; [done|]. split!. naive_solver.
+        + move: ri xi Hi x' Hsat sr1' e' Hri HR1. apply: pp_to_all_forall_2.
           apply: pp_to_all_mono; [by apply: HR2N|].
-          move => [[??]?] ? /= Hcont ????.
-          have {}Hcont := Hcont _ _ ltac:(done) ltac:(done). destruct_all?.
+          move => [[??]?] ? /= Hcont ??????.
+          have {}Hcont := Hcont _ _ _ ltac:(done) ltac:(done) ltac:(done). destruct_all?.
           destruct e; simplify_eq/=.
           tstep_s. eexists (Some (Outgoing, _)). split!; [done|].
           apply: steps_spec_step_end; [done|] => ??.
           tstep_s.
-          apply: pp_to_ex_mono_res; [done..|].
           apply: pp_to_ex_mono; [done|].
-          move => [[??]?] ? /= ????. destruct_all?; simplify_eq. split!.
-          apply: Hloop; [done|]. split!; [naive_solver|done..].
+          move => [[??]?] ? /= ?. destruct_all?; simplify_eq. split!; [done|].
+          apply: Hloop; [done|]. split!. naive_solver.
     Qed.
 
   Lemma mod_prepost_combine
@@ -712,18 +631,24 @@ Section prepost.
         INV Env s1 s2 s x1 x2 x →
        (∀ s1 s2 s x1 x2 x e,
            INV Env s1 s2 s x1 x2 x →
-           pp_to_all (i e s) x (λ r y,
-             pp_to_ex (i1 e s1) x1 (λ r1 y1,
-               pp_to_ex (i2 r1.1 s2) x2 (λ r2 y2,
+           pp_to_all (i e s) (λ r y, ∀ x',
+            satisfiable (x ∗ y ∗ x') →
+             pp_to_ex (i1 e s1) (λ r1 y1, ∃ x1',
+               satisfiable (x1 ∗ y1 ∗ x1') ∧
+               pp_to_ex (i2 r1.1 s2) (λ r2 y2, ∃ x2',
+                 satisfiable (x2 ∗ y2 ∗ x2') ∧
                  r.1 = r2.1 ∧
-                 INV Prog r1.2 r2.2 r.2 y1 y2 y)))) →
+                 INV Prog r1.2 r2.2 r.2 x1' x2' x')))) →
        (∀ s1 s2 s x1 x2 x e,
            INV Prog s1 s2 s x1 x2 x →
-           pp_to_all (o2 e s2) x2 (λ r2 y2,
-             pp_to_all (o1 r2.1 s1) x1 (λ r1 y1,
-               pp_to_ex (o e s) x (λ r y,
+           pp_to_all (o2 e s2) (λ r2 y2, ∀ x2',
+             satisfiable (x2' ∗ y2 ∗ x2) →
+             pp_to_all (o1 r2.1 s1) (λ r1 y1, ∀ x1',
+             satisfiable (x1' ∗ y1 ∗ x1) →
+               pp_to_ex (o e s) (λ r y, ∃ x',
+                 satisfiable (x' ∗ y ∗ x) ∧
                  r.1 = r1.1 ∧
-                 INV Env r1.2 r2.2 r.2 y1 y2 y)))) →
+                 INV Env r1.2 r2.2 r.2 x1' x2' x')))) →
     trefines (MS ((mod_prepost i1 o1 (mod_prepost i2 o2 m)) )
                  (SMFilter, (SMFilter, σ, (PPOutside, s2, x2)), (PPOutside, s1, x1)))
              (MS (mod_prepost i o m)
@@ -745,10 +670,10 @@ Section prepost.
       move => [[σf {}σ] [[σpp {}s] {}x]] ?. destruct_all?; simplify_eq.
       - tstep_i => ?.
         tstep_s. split!.
-        tstep_s. apply: pp_to_all_mono; [by apply: Henv|]. move => r y /= ?.
-        tstep_i. apply: pp_to_ex_mono; [done|]. move => r1 y1 /= ?.
+        tstep_s. apply: pp_to_all_mono; [by apply: Henv|]. move => r y /= ???.
+        tstep_i. apply: pp_to_ex_mono; [naive_solver|]. move => r1 y1 /= [?[??]]. split!; [done|].
         tstep_i => ??. subst.
-        tstep_i. apply: pp_to_ex_mono; [done|]. move => r2 y2 /= [??].
+        tstep_i. apply: pp_to_ex_mono; [done|]. move => r2 y2 /= [?[?[??]]]. split!; [done|].
         apply: Hloop; [done|]. split!. by f_equal.
       - tstep_both.
         apply steps_impl_step_end => κ Pσ2 ? *. destruct κ as [e'|]. 2: {
@@ -757,10 +682,10 @@ Section prepost.
           apply: Hloop; [done|]. by split!.
         }
         tend. have [σ' Hσ'] := vis_no_all _ _ _ ltac:(done). eexists σ'. split; [naive_solver|].
-        tstep_i. apply: pp_to_all_mono; [by apply: Hprog|]. move => r2 y2 /= ?.
-        tstep_i. apply: pp_to_all_mono; [done|]. move => r1 y1 /= ?.
+        tstep_i. apply: pp_to_all_mono; [by apply: Hprog|]. move => r2 y2 /= ???.
+        tstep_i. apply: pp_to_all_mono; [naive_solver|]. move => r1 y1 /= ???.
         tstep_s. eexists _. apply: steps_spec_step_end; [done|] => ?? /=.
-        tstep_s. apply: pp_to_ex_mono; [done|]. move => r y /= [??]. split!.
+        tstep_s. apply: pp_to_ex_mono; [naive_solver|]. move => r y /= [?[?[??]]]. split!; [done|].
         apply: Hloop; [done|]. split!. naive_solver.
       - tstep_both.
         apply steps_impl_step_end => κ Pσ2 ? *. destruct κ as [e'|]. 2: {
@@ -773,4 +698,80 @@ Section prepost.
         apply: steps_spec_step_end; [done|] => ??. tend. split!; [done|].
         apply: Hloop; [done|]. split!.
     Qed.
+
+  Lemma mod_prepost_impl
+        {EV1 EV2 Si Ss : Type}
+        {Mi Ms : ucmra}
+        (m : module EV2)
+        (INV : player → Si → Ss → uPred Mi → uPred Ms → Prop)
+        (i_i : EV1 → Si → prepost (EV2 * Si) Mi)
+        (o_i : EV2 → Si → prepost (EV1 * Si) Mi)
+        (i_s : EV1 → Ss → prepost (EV2 * Ss) Ms)
+        (o_s : EV2 → Ss → prepost (EV1 * Ss) Ms)
+        σ si ss xi xs
+        `{!VisNoAll m}
+        :
+        INV Env si ss xi xs →
+       (∀ si ss xi xs e,
+           INV Env si ss xi xs →
+           pp_to_all (i_s e ss) (λ rs ys, ∀ xs',
+            satisfiable (xs ∗ ys ∗ xs') →
+             pp_to_ex (i_i e si) (λ ri yi, ∃ xi',
+               satisfiable (xi ∗ yi ∗ xi') ∧
+               rs.1 = ri.1 ∧
+               INV Prog ri.2 rs.2 xi' xs'))) →
+       (∀ si ss xi xs e,
+           INV Prog si ss xi xs →
+           pp_to_all (o_i e si) (λ ri yi, ∀ xi',
+             satisfiable (xi' ∗ yi ∗ xi) →
+             pp_to_ex (o_s e ss) (λ rs ys, ∃ xs',
+               satisfiable (xs' ∗ ys ∗ xs) ∧
+               rs.1 = ri.1 ∧
+               INV Env ri.2 rs.2 xi' xs'))) →
+    trefines (MS ((mod_prepost i_i o_i m) )
+                 (SMFilter, σ, (PPOutside, si, xi)))
+             (MS (mod_prepost i_s o_s m)
+                 (SMFilter, σ, (PPOutside, ss, xs))).
+    Proof.
+      move => Hinv Henv Hprog.
+      apply tsim_implies_trefines => /= n.
+      unshelve apply: tsim_remember. { simpl. exact (λ _
+          '(σfi, σi, (σppi, si, xi))
+          '(σfs, σs, (σpps, ss, xs)),
+           ∃ p, σi = σs ∧ INV p si ss xi xs ∧ σfi = σfs ∧ σppi = σpps ∧
+           ((p = Env ∧ σfi = SMFilter ∧ σppi = PPOutside) ∨
+            (p = Prog ∧ σppi = PPInside ∧
+               (σfi = SMProg ∨ ∃ e, σfi = SMProgRecv e)))). }
+      { split!. } { done. }
+      move => {}n _ /= Hloop {Hinv}.
+      move => [[σfi σi] [[σppi {}si] {}xi]].
+      move => [[σfs {}σs] [[σpps {}ss] {}xs]] ?. destruct_all?; simplify_eq.
+      - tstep_i => ?.
+        tstep_s. split!.
+        tstep_s. apply: pp_to_all_mono; [by apply: Henv|]. move => r y /= ???.
+        tstep_i. apply: pp_to_ex_mono; [naive_solver|]. move => r1 y1 /= [?[??]]. split!; [done|]. destruct_all?.
+        apply: Hloop; [done|]. split!. by f_equal.
+      - tstep_both.
+        apply steps_impl_step_end => κ Pσ2 ? *. destruct κ as [e'|]. 2: {
+          tstep_s. eexists None.
+          apply: steps_spec_step_end; [done|] => ??. tend. eexists _. split; [done|].
+          apply: Hloop; [done|]. by split!.
+        }
+        tend. have [σ' Hσ'] := vis_no_all _ _ _ ltac:(done). eexists σ'. split; [naive_solver|].
+        tstep_i. apply: pp_to_all_mono; [by apply: Hprog|]. move => r2 y2 /= ???.
+        tstep_s. eexists _. apply: steps_spec_step_end; [done|] => ?? /=.
+        tstep_s. apply: pp_to_ex_mono; [naive_solver|]. move => r y /= [?[?[??]]]. split!; [done|].
+        apply: Hloop; [done|]. split!. naive_solver.
+      - tstep_both.
+        apply steps_impl_step_end => κ Pσ2 ? *. destruct κ as [e'|]. 2: {
+          tstep_s. eexists None. split!.
+          apply: steps_spec_step_end; [done|] => ??. tend. eexists _. split; [done|].
+          apply: Hloop; [done|]. by split!.
+        }
+        move => ->.
+        tstep_s. eexists (Some _). split; [done|].
+        apply: steps_spec_step_end; [done|] => ??. tend. split!; [done|].
+        apply: Hloop; [done|]. split!.
+    Qed.
+
 End prepost.
