theories/imp.v
@@ -948,11 +948,12 @@ Inductive imp_prepost_proof_stack {S} {M : ucmra} (n : trace_index) (fnsi fnss :
   imp_prepost_proof_stack n fnsi fnss i o R b s0 r0 Ki Ks →
   (∀ hi vi s2 (r2 : uPred M),
       R true (s1, r1) (s2, r2) →
-      pp_to_all (i (Incoming, EIReturn vi hi) s2) r2 (λ '(e', s3) r3,
+      pp_to_all (i (Incoming, EIReturn vi hi) s2) (λ '(e', s3) r3, ∀ r3',
+      satisfiable (r2 ∗ r3 ∗ r3') →
       ∃ vs hs, e' = (Incoming, EIReturn vs hs) ∧
       Imp (expr_fill (Ki' ++ Ki) (Val vi)) hi fnsi
-        ⪯{imp_module, mod_prepost (S:=S) i o imp_module, n, true}
-        (SMProg, Imp (expr_fill (Ks' ++ Ks) (Val vs)) hs fnss, (PPInside, s3, r3)))) →
+        ⪯{imp_module, mod_prepost (M:=M) (S:=S) i o imp_module, n, true}
+        (SMProg, Imp (expr_fill (Ks' ++ Ks) (Val vs)) hs fnss, (PPInside, s3, r3')))) →
   imp_prepost_proof_stack n fnsi fnss i o R true s1 r1 (Ki' ++ Ki) (Ks' ++ Ks)
 .
 
@@ -963,7 +964,8 @@ Lemma imp_prepost_proof_stack_mono S M n n' fns1 fns2 i o R s r b Ki Ks:
 Proof.
   move => Hs. elim: Hs n'; [by econs|].
   move => *. econs; [naive_solver|] => *.
-  apply: pp_to_all_mono; [naive_solver|]. move => [??] ??. destruct_all?; subst. split!.
+  apply: pp_to_all_mono; [naive_solver|]. move => [??] ? Hsim ??.
+  move: Hsim => /(_ _ ltac:(done))?. destruct_all?; subst. split!.
   by apply: tsim_mono.
 Qed.
 
@@ -974,7 +976,7 @@ Lemma imp_prepost_proof_stack_mono_R M S n fns1 fns2 i o R s s' r r' b Ki Ks `{!
 Proof.
   move => Hs. elim: Hs s'; [by econs|].
   move => ??????????? Hcont ??. econs; [naive_solver|] => *.
-  apply: pp_to_all_mono. { apply Hcont. by etrans. } done.
+  apply: pp_to_all_mono. { apply: Hcont. by etrans. } done.
 Qed.
 
 Lemma imp_prepost_proof {S} {M : ucmra} R `{!∀ b, PreOrder (R b)} i o fns1 fns2 s0 (r0 : uPred M):
@@ -983,7 +985,8 @@ Lemma imp_prepost_proof {S} {M : ucmra} R `{!∀ b, PreOrder (R b)} i o fns1 fns
   (∀ n K1 K2 f fn1 vs1 h1 s1 r1,
       R false (s0, r0) (s1, r1) →
       fns1 !! f = Some fn1 →
-      pp_to_all (i (Incoming, EICall f vs1 h1) s1) r1 (λ '(e', s2) r2,
+      pp_to_all (i (Incoming, EICall f vs1 h1) s1) (λ '(e', s2) r2, ∀ r2',
+      satisfiable (r1 ∗ r2 ∗ r2') →
       ∃ vs2 h2 fn2, e' = (Incoming, EICall f vs2 h2) ∧ fns2 !! f = Some fn2 ∧ (
         length vs2 = length (fd_args fn2) →
           length vs1 = length (fd_args fn1) ∧ (
@@ -994,14 +997,16 @@ Lemma imp_prepost_proof {S} {M : ucmra} R `{!∀ b, PreOrder (R b)} i o fns1 fns
          fns2 !! f = None →
          Forall2 (λ e v, e = Val v) es1 vs1' →
          Forall2 (λ e v, e = Val v) es2 vs2' →
-         pp_to_ex (o (Outgoing, EICall f vs2' h2') s3) r3 (λ '(e''', s4) r4,
-            e''' = (Outgoing, EICall f vs1' h1') ∧ R false (s1, r1) (s4, r4) ∧
-           ∀ v1'' h1'' s5 r5, R true (s4, r4) (s5, r5) →
-                   pp_to_all (i (Incoming, EIReturn v1'' h1'') s5) r5 (λ '(e''''', s6) r6,
+         pp_to_ex (o (Outgoing, EICall f vs2' h2') s3) (λ '(e''', s4) r4, ∃ r4',
+            e''' = (Outgoing, EICall f vs1' h1') ∧ R false (s1, r1) (s4, r4') ∧
+            satisfiable (r4' ∗ r4 ∗ r3) ∧
+           ∀ v1'' h1'' s5 r5, R true (s4, r4') (s5, r5) →
+                   pp_to_all (i (Incoming, EIReturn v1'' h1'') s5) (λ '(e''''', s6) r6, ∀ r6',
+                     satisfiable (r5 ∗ r6 ∗ r6') →
             ∃ v2'' h2'', e''''' = (Incoming, EIReturn v2'' h2'') ∧
           Imp (expr_fill K1 (expr_fill K1' (Val v1''))) h1'' fns1
               ⪯{imp_module, mod_prepost i o imp_module, n', true}
-          (SMProg, Imp (expr_fill K2 (expr_fill K2' (Val v2''))) h2'' fns2, (PPInside, s6, r6)))) →
+          (SMProg, Imp (expr_fill K2 (expr_fill K2' (Val v2''))) h2'' fns2, (PPInside, s6, r6')))) →
 
           Imp (expr_fill K1 (expr_fill K1' (Call f es1))) h1' fns1
               ⪯{imp_module, mod_prepost i o imp_module, n', b}
@@ -1009,14 +1014,14 @@ Lemma imp_prepost_proof {S} {M : ucmra} R `{!∀ b, PreOrder (R b)} i o fns1 fns
       (* Return *)
       (∀ n' v1 v2 h1' h2' b s3 r3,
          n' ⊆ n →
-         pp_to_ex (o (Outgoing, EIReturn v2 h2') s3) r3 (λ '(e''', s4) r4,
-               e''' = (Outgoing, EIReturn v1 h1') ∧ R true (s1, r1) (s4, r4)) →
+         pp_to_ex (o (Outgoing, EIReturn v2 h2') s3) (λ '(e''', s4) r4, ∃ r4',
+               e''' = (Outgoing, EIReturn v1 h1') ∧ R true (s1, r1) (s4, r4') ∧ satisfiable (r4' ∗ r4 ∗ r3)) →
           Imp (expr_fill K1 (Val v1)) h1' fns1
               ⪯{imp_module, mod_prepost i o imp_module, n', b}
           (SMProg, Imp (expr_fill K2 (Val v2)) h2' fns2, (PPInside, s3, r3))) →
       Imp (expr_fill K1 (subst_l fn1.(fd_args) vs1 fn1.(fd_body))) h1 fns1
           ⪯{imp_module, mod_prepost i o imp_module, n, false}
-          (SMProg, Imp (expr_fill K2 (subst_l fn2.(fd_args) vs2 fn2.(fd_body))) h2 fns2, (PPInside, s2, r2)))))) →
+          (SMProg, Imp (expr_fill K2 (subst_l fn2.(fd_args) vs2 fn2.(fd_body))) h2 fns2, (PPInside, s2, r2')))))) →
   trefines (MS imp_module (initial_imp_state fns1))
            (MS (mod_prepost (S:=S) i o imp_module)
                (SMFilter, initial_imp_state fns2, (PPOutside, s0, r0))).
@@ -1043,7 +1048,7 @@ Proof.
   tstep_i. split => *.
   - tstep_s. split!.
     tstep_s. apply: pp_to_all_mono. { by eapply (Hcall n (ReturnExtCtx b :: Ki) (ReturnExtCtx b :: Ks)). }
-    move => -[??] ? [?[?[?[?[? Hcall']]]]]. simplify_eq/=.
+    move => -[??] ? Hcall' ??. move: Hcall' => /(_ _ ltac:(done))[?[?[?[?[? Hcall']]]]]. simplify_eq/=.
     tstep_s. left. split!. repeat case_bool_decide; try by tstep_s. 2: naive_solver.
     have [//|? {}Hcall'] := Hcall'. apply: tsim_mono_b. apply: Hcall'.
     + move => n' f K1' K2' es1 es2 vs1' vs2' ???????? Hall1 Hall2 ?.
@@ -1051,15 +1056,15 @@ Proof.
       have ?: es2 = Val <$> vs2'. { clear -Hall2. elim: Hall2; naive_solver. } subst.
       tstep_i. split => *; simplify_eq. rewrite orb_true_r. tstep_s. right. split!.
       tstep_s. apply: pp_to_ex_mono; [done|].
-      move => [??] ? /= [?[??]]. simplify_eq. split!.
+      move => [??] ? /= [?[?[?[??]]]]. simplify_eq. split!; [done|].
       apply: Hloop; [done|].
       split!; [done..|by etrans|].
       econs; [by apply: imp_prepost_proof_stack_mono|].
       move => ?????. apply: pp_to_all_mono; [naive_solver|].
-      move => [??] ? /= ?. destruct_all?. subst. split!.
+      move => [??] ? /= Hsim ??. move: Hsim => /(_ _ ltac:(done))?. destruct_all?. subst. split!.
       rewrite !expr_fill_app /=. done.
     + move => *. tstep_s. tstep_i. rewrite orb_true_r. tstep_s. apply: pp_to_ex_mono; [done|].
-      move => [??] ? [-> ?] /=. split!. apply: tsim_mono; [|done]. apply: Hloop; [done|].
+      move => [??] ? [?[?[??]]] /=. subst. split!; [done|]. apply: tsim_mono; [|done]. apply: Hloop; [done|].
       split!. 1, 2: done.
       { etrans; [done|]. by apply: HR. }
       { by apply: imp_prepost_proof_stack_mono_R. }
@@ -1067,7 +1072,7 @@ Proof.
     inversion Hs; clear Hs; simplify_eq/= => //.
     tstep_s. split!.
     tstep_s. apply: pp_to_all_mono; [naive_solver|].
-    move => [??] ? [?[?[? Hsim]]]; simplify_eq/=.
+    move => [??] ? Hsim ??. move: Hsim => /(_ _ ltac:(done))?. destruct_all?. simplify_eq/=.
     tstep_s. right. split!.
 Qed.
 
