theories/satisfiable.v
@@ -1,0 +1,229 @@
+Require Export iris.algebra.cmra.
+Require Export iris.algebra.updates.
+Require Export iris.base_logic.base_logic.
+Require Export iris.proofmode.proofmode.
+Require Import iris.proofmode.environments.
+Require Import iris.proofmode.reduction.
+
+Section satisfiable.
+  Context {M : ucmra}.
+
+  Definition satisfiable (P: uPred M) := ∃ x : M, ✓{0} x ∧ uPred_holds P 0 x.
+
+  Global Instance satisfiable_proper : Proper ((≡) ==> iff) satisfiable.
+  Proof.
+    move => ?? Hequiv. unfold satisfiable. f_equiv => ?.
+    split => -[??]. all: split; [done|]. all: apply: uPred_holds_ne; [| |done..]; [|done]; by rewrite Hequiv.
+  Qed.
+
+  Lemma satisfiable_valid x:
+    satisfiable (uPred_ownM x) → ✓{0} x.
+  Proof. unfold satisfiable; uPred.unseal. move => [?[??]]. by apply: cmra_validN_includedN. Qed.
+
+  Lemma satisfiable_mono x y:
+    satisfiable x →
+    (x ⊢ y) →
+    satisfiable y.
+  Proof. move => [?[??]] Hentails. eexists _. split; [done|]. by apply Hentails. Qed.
+
+  Lemma satisfiable_emp_valid y:
+    (⊢ y) →
+    satisfiable y.
+  Proof.
+    move => Hentails.
+    apply: satisfiable_mono; [|done].
+    unfold satisfiable; uPred.unseal.
+    eexists ε. split; [|done].
+    apply ucmra_unit_validN.
+  Qed.
+
+  Lemma satisfiable_pure_1 (ϕ : Prop):
+    ϕ →
+    satisfiable ⌜ϕ⌝.
+  Proof. move => ?. apply satisfiable_emp_valid. by iPureIntro. Qed.
+
+  Lemma satisfiable_pure_2 (ϕ : Prop):
+    satisfiable ⌜ϕ⌝ →
+    ϕ.
+  Proof. unfold satisfiable; uPred.unseal. naive_solver. Qed.
+
+  Lemma satisfiable_exist_1 {A} P:
+    (∃ x : A, satisfiable (P x)) →
+    satisfiable (∃ x, P x).
+  Proof. move => [??]. apply: satisfiable_mono; [done|]. iIntros "?". by iExists _. Qed.
+
+  Lemma satisfiable_exist_2 {A} P:
+    satisfiable (∃ x, P x) →
+    ∃ x : A, satisfiable (P x).
+  Proof. unfold satisfiable; uPred.unseal. move => [? [? [??]]]. naive_solver. Qed.
+
+  Lemma satisfiable_sep_2 P1 P2:
+    satisfiable (P1 ∗ P2) →
+    satisfiable P1 ∧ satisfiable P2.
+  Proof. move => ?. split; (apply: satisfiable_mono; [done|]); by iIntros "[??]". Qed.
+
+  Lemma satisfiable_and_2 P1 P2:
+    satisfiable (P1 ∧ P2) →
+    satisfiable P1 ∧ satisfiable P2.
+  Proof. move => ?. split; (apply: satisfiable_mono; [done|]); eauto using bi.and_elim_l, bi.and_elim_r. Qed.
+
+  Lemma satisfiable_bupd_2 x:
+    satisfiable (|==> x) →
+    satisfiable x.
+  Proof.
+    unfold satisfiable; uPred.unseal.
+    move => -[x'[Hv HP]].
+    destruct (HP 0 ε) as [y HP']; [done|by rewrite right_id|].
+    move: HP'. rewrite right_id; eauto.
+  Qed.
+
+  Lemma satisfiable_bmono x y:
+    satisfiable x →
+    (x ==∗ y) →
+    satisfiable y.
+  Proof. move => ??. apply satisfiable_bupd_2. by apply: satisfiable_mono. Qed.
+
+  Lemma satisfiable_init x y:
+    ✓ x →
+    (uPred_ownM x ==∗ y) →
+    satisfiable y.
+  Proof.
+    move => /cmra_valid_validN Hvalid Hentails.
+    apply: satisfiable_bmono; [|done].
+    unfold satisfiable; uPred.unseal.
+    eexists x. split; [done|]. rewrite /uPred_holds/=. done.
+  Qed.
+
+  (* The following two lemmas don't seem provable. But they would be
+  very useful to be able to use frame preserving updates in the
+  prepost because this would allow concurrency. (i.e. in the
+  postcondition require proving an frame preserving update from the
+  initial predicate.) But for this, one always needs to maintain a P1
+  ==∗ P_cur during the proof and that seems annoying without the
+  lemmas below. An idea would be to add angelic steps that allow
+  updating the P1 at arbitrary points with a bupd but that seems a bit
+  annoying to add.
+
+  See 083546b88cf853dad1f06a8d819059f5c20fc708 for the framepreserving
+ update approach *)
+  (*
+  Lemma sat_wand_ex A P1 P2 :
+    satisfiable P1 →
+    (P1 -∗ ∃ x : A, P2 x) →
+    ∃ x, (P1 -∗ P2 x).
+  Proof.
+    move => /satisfiable_mono Hsat Hw. move: (Hsat _ Hw) => /satisfiable_exist_2[??].
+
+  Lemma sat_exist P1 P2 (φ : Prop) :
+    (P1 ==∗ P2) →
+    satisfiable P1 →
+    (P2 ==∗ ∃ P3, P3 ∗ ⌜(P1 ==∗ P3) → φ⌝) →
+    φ.
+  Proof.
+    move => Hw1 Hsat Hw2.
+    have Hw3 : (P1 ==∗ ∃ P3, P3 ∗ ⌜(P1 ==∗ P3) → φ⌝).
+    { etrans; [done|]. iIntros ">?". by iApply Hw2. }
+    *)
+
+
+End satisfiable.
+
+
+Section tactics.
+  Context {M : ucmra}.
+  Implicit Types (P : uPred M).
+
+  Definition iSat_end (Φ : Prop) : uPred M :=
+    ∃ P', P' ∗ ⌜satisfiable P' → Φ⌝.
+
+  Lemma sat_start_intro_tac P (Φ : Prop) :
+    satisfiable P →
+    (P -∗ iSat_end Φ) →
+    Φ.
+  Proof.
+    move => /satisfiable_mono/[apply].
+    move => /satisfiable_exist_2[?]/satisfiable_sep_2[?/satisfiable_pure_2].
+    by apply.
+  Qed.
+End tactics.
+
+Definition sat_of_envs {PROP : bi} (Δ : envs PROP) : PROP := of_envs Δ.
+Global Arguments sat_of_envs : simpl never.
+
+Section tactics.
+Context {PROP : bi}.
+Implicit Types Γ : env PROP.
+Implicit Types Δ : envs PROP.
+Implicit Types P Q : PROP.
+Lemma tac_sat_accu Δ P :
+  sat_of_envs Δ = P →
+  envs_entails Δ P.
+Proof. rewrite envs_entails_eq=><-. done. Qed.
+
+Lemma tac_sat_start_proof Δ P :
+  envs_entails Δ P →
+  sat_of_envs Δ -∗ P.
+Proof. rewrite envs_entails_eq=><-. done. Qed.
+
+End tactics.
+
+Notation "Γ '--------------------------------------' □ Δ '--------------------------------------' ∗ " :=
+  (sat_of_envs (Envs Γ Δ _))
+  (at level 1, left associativity,
+  format "'[' Γ '--------------------------------------' □ '//' Δ '--------------------------------------' ∗ ']'", only printing) :
+  stdpp_scope.
+Notation "Δ '--------------------------------------' ∗ " :=
+  (sat_of_envs (Envs Enil Δ _))
+  (at level 1, left associativity,
+  format "'[' Δ '--------------------------------------' ∗ ']'", only printing) : stdpp_scope.
+Notation "Γ '--------------------------------------' □ " :=
+  (sat_of_envs (Envs Γ Enil _))
+  (at level 1, left associativity,
+  format "'[' Γ '--------------------------------------' □ ']'", only printing)  : stdpp_scope.
+Notation "'--------------------------------------' ∗" := (sat_of_envs (Envs Enil Enil _))
+  (at level 1, format "'[' '--------------------------------------' ∗ ']'", only printing) : stdpp_scope.
+
+
+(** internal tactics *)
+Ltac iSatStartProof :=
+  lazymatch goal with
+  | |- sat_of_envs _ -∗ _ => apply tac_sat_start_proof
+  | _ => idtac
+  end.
+Tactic Notation "iSatAccu" :=
+  iStartProof; eapply tac_sat_accu; [pm_reflexivity || fail "iSatAccu: not an evar"].
+
+(** tactics for the user *)
+Tactic Notation "iSatStart" ident(H) :=
+  apply (sat_start_intro_tac _ _ H); clear H; iSatStartProof.
+Tactic Notation "iSatStart" :=
+  lazymatch goal with
+  | H1 : satisfiable _, H2 : satisfiable _ |- _ => fail "Multiple satisfiable! Pick one via iSatStart H."
+  | H : satisfiable _ |- _ => iSatStart H
+  end.
+
+Ltac iSatStop :=
+  lazymatch goal with
+  | |- environments.envs_entails _ (iSat_end _) =>
+      iExists _; iSplitL; [iSatAccu|iPureIntro => ?]
+  | |- _ => fail "unknown goal!"
+  end.
+
+Ltac iSatClear :=
+  repeat match goal with | H : satisfiable _ |- _ => clear H end.
+
+Tactic Notation "iSatMono" ident(H) :=
+  apply (satisfiable_mono _ _ H); iSatStartProof.
+Tactic Notation "iSatMono" :=
+  lazymatch goal with
+  | H1 : satisfiable _, H2 : satisfiable _ |- _ => fail "Multiple satisfiable! Pick one via iSatMono H"
+  | H : satisfiable _ |- _ => iSatMono H
+  end.
+
+Tactic Notation "iSatMonoBupd" ident(H) :=
+  apply (satisfiable_bmono _ _ H); iSatStartProof.
+Tactic Notation "iSatMonoBupd" :=
+  lazymatch goal with
+  | H1 : satisfiable _, H2 : satisfiable _ |- _ => fail "Multiple satisfiable! Pick one via iSatMonoBupd H"
+  | H : satisfiable _ |- _ => iSatMonoBupd H
+  end.
